cedar-lean/Cedar/Spec/PartialValue.lean
@@ -16,6 +16,7 @@
 
 import Cedar.Data.Map
 import Cedar.Spec.Ext.IPAddr
+import Cedar.Spec.ExtFun
 import Cedar.Spec.PartialExpr
 import Cedar.Spec.Value
 
@@ -33,19 +34,35 @@ inductive PartialValue where
 
 deriving instance Repr, DecidableEq, Inhabited for PartialValue
 
-def Value.asPartialExpr (v : Value) : PartialExpr :=
-  match v with
-  | .prim p => PartialExpr.lit p
-  | .set s => PartialExpr.set (s.elts.map Value.asPartialExpr)
-  | .record m => PartialExpr.record (m.kvs.map fun (k, v)=> (k, v.asPartialExpr))
-  | .ext (.decimal d) => PartialExpr.call ExtFun.decimal [PartialExpr.lit (.string d.unParse)]
-  | .ext (.ipaddr ip) => PartialExpr.call ExtFun.ip [PartialExpr.lit (.string (Cedar.Spec.Ext.IPAddr.unParse ip))]
-decreasing_by sorry
-
 def PartialValue.asPartialExpr (v : PartialValue) : PartialExpr :=
   match v with
-  | .value v    => Value.asPartialExpr v
+  | .value v    => v.asPartialExpr
   | .residual r => r
+
+/--
+  Like `PartialValue`, but cannot contain residual expressions which depend on
+  vars or entity data
+-/
+inductive RestrictedPartialValue where
+  | value (v : Value)
+  | residual (r : RestrictedPartialExpr)
+
+deriving instance Inhabited for RestrictedPartialValue
+
+def RestrictedPartialValue.asPartialExpr (v : RestrictedPartialValue) : PartialExpr :=
+  match v with
+  | .value v    => v.asPartialExpr
+  | .residual r => r.asPartialExpr
+
+def RestrictedPartialValue.asRestrictedPartialExpr (v : RestrictedPartialValue) : RestrictedPartialExpr :=
+  match v with
+  | .value v    => v.asRestrictedPartialExpr
+  | .residual r => r
+
+def RestrictedPartialValue.asPartialValue (v : RestrictedPartialValue) : PartialValue :=
+  match v with
+  | .value v    => .value v
+  | .residual r => .residual (r.asPartialExpr)
 
 /--
   Given a map of unknown-name to value, substitute all unknowns with the
@@ -55,7 +72,7 @@ def PartialValue.asPartialExpr (v : PartialValue) : PartialExpr :=
 -/
 -- NB: this function can't live in PartialExpr.lean because it needs PartialValue, and
 -- PartialExpr.lean can't import PartialValue, cyclic dependency
-def PartialExpr.subst (x : PartialExpr) (subsmap : Map String PartialValue) : PartialExpr :=
+def PartialExpr.subst (x : PartialExpr) (subsmap : Map String RestrictedPartialValue) : PartialExpr :=
   match x with
   | .lit _ => x -- no unknowns, nothing to substitute
   | .var _ => x -- no unknowns, nothing to substitute
@@ -101,14 +118,150 @@ decreasing_by sorry
 
 /--
   Given a map of unknown-name to value, substitute all unknowns with the
+  corresponding values, producing an Expr.
+  This means that `subsmap` must contain mappings for all the unknowns (or this
+  function will return `none`).
+-/
+-- NB: this function can't live in PartialExpr.lean because it needs PartialValue, and
+-- PartialExpr.lean can't import PartialValue, cyclic dependency
+def PartialExpr.fullSubst (x : PartialExpr) (subsmap : Map String Value) : Option Expr :=
+  match x with
+  | .lit p => some (.lit p)
+  | .var v => some (.var v)
+  | .ite x₁ x₂ x₃ => do
+    let x₁' ← x₁.fullSubst subsmap
+    let x₂' ← x₂.fullSubst subsmap
+    let x₃' ← x₃.fullSubst subsmap
+    some (.ite x₁' x₂' x₃')
+  | .and x₁ x₂ => do
+    let x₁' ← x₁.fullSubst subsmap
+    let x₂' ← x₂.fullSubst subsmap
+    some (.and x₁' x₂')
+  | .or x₁ x₂ => do
+    let x₁' ← x₁.fullSubst subsmap
+    let x₂' ← x₂.fullSubst subsmap
+    some (.or x₁' x₂')
+  | .unaryApp op x₁ => do
+    let x₁' ← x₁.fullSubst subsmap
+    some (.unaryApp op x₁')
+  | .binaryApp op x₁ x₂ => do
+    let x₁' ← x₁.fullSubst subsmap
+    let x₂' ← x₂.fullSubst subsmap
+    some (.binaryApp op x₁' x₂')
+  | .getAttr x₁ attr => do
+    let x₁' ← x₁.fullSubst subsmap
+    some (.getAttr x₁' attr)
+  | .hasAttr x₁ attr => do
+    let x₁' ← x₁.fullSubst subsmap
+    some (.hasAttr x₁' attr)
+  | .set xs => do
+    let xs' ← xs.mapM (PartialExpr.fullSubst · subsmap)
+    some (.set xs')
+  | .record pairs => do
+    let pairs' ← pairs.mapM λ (k, v) => v.fullSubst subsmap >>= λ v' => some (k, v')
+    some (.record pairs')
+  | .call xfn xs => do
+    let xs' ← xs.mapM (PartialExpr.fullSubst · subsmap)
+    some (.call xfn xs')
+  | unknown name => match subsmap.find? name with
+    | some val => val.asExpr
+    | none => none -- no substitution available, return `none`
+decreasing_by sorry
+
+/--
+  Given a map of unknown-name to value, substitute all unknowns with the
+  corresponding values, producing a new RestrictedPartialExpr.
+  It's fine for some unknowns to not be in `subsmap`, in which case the returned
+  `RestrictedPartialExpr` will still contain some unknowns.
+-/
+-- NB: this function can't live in PartialExpr.lean because it needs RestrictedPartialValue,
+-- and PartialExpr.lean can't import RestrictedPartialValue, cyclic dependency
+def RestrictedPartialExpr.subst (x : RestrictedPartialExpr) (subsmap : Map String RestrictedPartialValue) : RestrictedPartialExpr :=
+  match x with
+  | .lit p => .lit p
+  | .set xs => .set (xs.map (RestrictedPartialExpr.subst · subsmap))
+  | .record attrs => .record (attrs.map λ (k, v) => (k, v.subst subsmap))
+  | .call xfn args => .call xfn args
+  | .unknown name => match subsmap.find? name with
+    | some val => val.asRestrictedPartialExpr
+    | none => x -- no substitution available, return `x` unchanged
+decreasing_by sorry
+
+mutual
+
+/--
+  Given a map of unknown-name to value, substitute all unknowns with the
+  corresponding values and fully evaluate, producing a Value.
+  This means that `subsmap` must contain mappings for all the unknowns (or this
+  function will return `none`).
+
+  Also returns `none` if an extension constructor fails to evaluate.
+-/
+-- NB: this function can't live in PartialExpr.lean because it needs RestrictedPartialValue,
+-- and PartialExpr.lean can't import RestrictedPartialValue, cyclic dependency
+def RestrictedPartialExpr.fullSubst (x : RestrictedPartialExpr) (subsmap : Map String Value) : Option Value :=
+  match x with
+  | .lit p => some (.prim p)
+  | .set xs => do
+      let xs' ← xs.mapM (RestrictedPartialExpr.fullSubst · subsmap)
+      some (.set (Set.make xs'))
+  | .record attrs => do
+      let attrs' ← attrs.mapM λ (k, v) => v.fullSubst subsmap >>= λ v' => some (k, v')
+      some (.record (Map.make attrs'))
+  | .call xfn args => match ExtFun.call xfn args with
+    | .ok v => some v
+    | .error _ => none
+  | .unknown name => subsmap.find? name -- if no substitution is available, returns `none`
+
+/--
+  Given a map of unknown-name to value, substitute all unknowns with the
   corresponding values, producing a new PartialValue.
   It's fine for some unknowns to not be in `subsmap`, in which case the returned
   `PartialValue` will still contain some unknowns.
 -/
-def PartialValue.subst (v : PartialValue) (subsmap : Map String PartialValue) : PartialValue :=
+def PartialValue.subst (v : PartialValue) (subsmap : Map String RestrictedPartialValue) : PartialValue :=
   match v with
   | .residual r => .residual (r.subst subsmap)
   | .value v    => .value v -- doesn't contain unknowns, nothing to substitute
+
+/- Hard to define PartialValue.fullSubst, because it could be an arbitrary residual depending on variables / entity data etc.
+  Probably should return Option Expr if we need this. But hopefully we can do without this.
+/--
+  Given a map of unknown-name to value, substitute all unknowns with the
+  corresponding values, producing a Value.
+  This means that `subsmap` must contain mappings for all the unknowns (or this
+  function will return `none`).
+-/
+def PartialValue.fullSubst (v : PartialValue) (subsmap : Map String Value) : Option Value :=
+  match v with
+  | .residual r => r.fullSubst subsmap
+  | .value v    => some v
+-/
+
+/--
+  Given a map of unknown-name to value, substitute all unknowns with the
+  corresponding values, producing a new RestrictedPartialValue.
+  It's fine for some unknowns to not be in `subsmap`, in which case the returned
+  `RestrictedPartialValue` will still contain some unknowns.
+-/
+def RestrictedPartialValue.subst (v : RestrictedPartialValue) (subsmap : Map String RestrictedPartialValue) : RestrictedPartialValue :=
+  match v with
+  | .residual r => .residual (r.subst subsmap)
+  | .value v    => .value v -- doesn't contain unknowns, nothing to substitute
+
+/--
+  Given a map of unknown-name to value, substitute all unknowns with the
+  corresponding values, producing a Value.
+  This means that `subsmap` must contain mappings for all the unknowns (or this
+  function will return `none`).
+-/
+def RestrictedPartialValue.fullSubst (v : RestrictedPartialValue) (subsmap : Map String Value) : Option Value :=
+  match v with
+  | .residual r => r.fullSubst subsmap
+  | .value v    => some v -- doesn't contain unknowns, nothing to substitute
+
+end
+decreasing_by sorry
 
 /--
   If converting a Value to PartialExpr gives a primitive, the Value was that
@@ -129,9 +282,16 @@ theorem Value.prim_prim {v : Value} {p : Prim} :
 /--
   subst on an Expr is id
 -/
-theorem subs_expr_id {expr : Expr} {subsmap : Map String PartialValue} :
+theorem subs_expr_id {expr : Expr} {subsmap : Map String RestrictedPartialValue} :
   expr.asPartialExpr.subst subsmap = expr.asPartialExpr
 := by
-  sorry
+  unfold PartialExpr.subst
+  cases expr <;> simp [Expr.asPartialExpr]
+  case and x₁ x₂ =>
+    -- inductive argument needed
+    sorry
+  all_goals {
+    sorry
+  }
 
 end Cedar.Spec
